LeanSysF/Term.lean
@@ -1,126 +1,124 @@
 
 import LeanSubst
 
-inductive Ctor2Kind where
-| app | tapp | arr
-
-inductive Bind1Kind where
-| tlam | all
-
-inductive Term where
-| star : Term
-| var : Nat -> Term
-| lam : Term -> Term -> Term
-| bind1 : Bind1Kind -> Term -> Term
-| ctor2 : Ctor2Kind -> Term -> Term -> Term
-
-inductive IsVar : Term -> Prop where
-| var : IsVar (.var x)
-
-def Var := { t : Term // IsVar t }
-
-inductive IsLam : Term -> Prop where
-| var : IsLam (.var x)
-| lam : IsLam A -> IsLam t -> IsLam (.lam A t)
-
-def Lam := {t : Term // IsLam t}
-
-namespace Var
-  def var (x : Nat) : Var := .mk (.var x) (by constructor)
-
-  @[simp]
-  def out : Var -> Nat
-  | .mk (.var x) _ => x
-end Var
-
-@[simp]
-instance instCoe_Var_Term : Coe Var Term where
-  coe := λ v => v.val
-
-protected def Term.repr (a : Term) (p : Nat) : Std.Format :=
-  match a with
-  | .star => "★"
-  | .var x => "#" ++ Nat.repr x
-  | .lam A t => "(λ[" ++ Term.repr A p ++ "] " ++ Term.repr t p ++ ")"
-  | .bind1 .all P => "(∀" ++ Term.repr P p ++  ")"
-  | .bind1 .tlam P => "(Λ" ++ Term.repr P p ++  ")"
-  | .ctor2 .app f a => "(" ++ Term.repr f p ++ " " ++ Term.repr a p ++ ")"
-  | .ctor2 .tapp f a => "(" ++ Term.repr f p ++ "·" ++ Term.repr a p ++ ")"
-  | .ctor2 .arr A B => "(" ++ Term.repr A p ++ " -> " ++ Term.repr B p ++ ")"
-
-instance : Repr Term where
-  reprPrec := Term.repr
-
-notation "★" => Term.star
-prefix:max "#" => Term.var
-notation:65 f:65 " :@ " a:64 => Term.ctor2 Ctor2Kind.app f a
-notation:65 f:65 " :@[" a "]" => Term.ctor2 Ctor2Kind.tapp f a
-notation ":λ[" A "] " t => Term.lam A t
-notation:64 A:63 " -:> " B:64 => Term.ctor2 Ctor2Kind.arr A B
-notation ":∀ " t => Term.bind1 Bind1Kind.all t
-notation "Λ " t => Term.bind1 Bind1Kind.tlam t
-
-namespace Term
-  @[simp]
-  def size : Term -> Nat
-  | ★ => 0
-  | .var _ => 0
-  | .lam A t => size A + size t + 1
-  | .bind1 _ t => size t + 1
-  | .ctor2 _ t1 t2 => size t1 + size t2 + 1
-end Term
-
 open LeanSubst
 
+inductive VariantSort where
+| bind | ctor
+
+inductive Variant : VariantSort -> Type where
+| star : Variant .ctor
+| app : Variant .ctor
+| tapp : Variant .ctor
+| arr : Variant .ctor
+| lam : Variant .bind
+| tlam : Variant .bind
+| all : Variant .bind
+
+@[reducible]
+def Variant.arity : Variant s -> Nat
+| star | tlam | all => 0
+| app | tapp | arr => 2
+| lam => 1
+
+inductive Term where
+| var : Nat -> Term
+| bind : (v : Variant .bind) -> (Fin v.arity -> Term) -> Term -> Term
+| ctor : (v : Variant .ctor) -> (Fin v.arity -> Term) -> Term
+
+-- protected def Term.repr (a : Term) (p : Nat) : Std.Format :=
+--   match a with
+--   | .star => "★"
+--   | .var x => "#" ++ Nat.repr x
+--   | .lam A t => "(λ[" ++ Term.repr A p ++ "] " ++ Term.repr t p ++ ")"
+--   | .bind1 .all P => "(∀" ++ Term.repr P p ++  ")"
+--   | .bind1 .tlam P => "(Λ" ++ Term.repr P p ++  ")"
+--   | .ctor2 .app f a => "(" ++ Term.repr f p ++ " " ++ Term.repr a p ++ ")"
+--   | .ctor2 .tapp f a => "(" ++ Term.repr f p ++ "·" ++ Term.repr a p ++ ")"
+--   | .ctor2 .arr A B => "(" ++ Term.repr A p ++ " -> " ++ Term.repr B p ++ ")"
+
+-- instance : Repr Term where
+--   reprPrec := Term.repr
+
+notation "★" => Term.ctor Variant.star mk0
+prefix:max "#" => Term.var
+notation:65 f:65 " :@ " a:64 => Term.ctor Variant.app (λ i => mk2 f a i)
+notation:65 f:65 " :@[" a "]" => Term.ctor Variant.tapp (λ i => mk2 f a i)
+notation ":λ[" A "] " t => Term.bind Variant.lam (λ i => mk1 A i) t
+notation:64 A:63 " -:> " B:64 => Term.ctor Variant.arr (λ i => mk2 A B i)
+notation ":∀ " t => Term.bind Variant.all mk0 t
+notation "Λ " t => Term.bind Variant.tlam mk0 t
 
 @[simp]
-def smap (lf : Subst.Lift Term) (f : Nat -> Subst.Action Term) : Term -> Term
-| ★ => ★
+instance : Inhabited Term where
+  default := ★
+
+@[coe]
+def Term.from_action : Subst.Action Term -> Term
+| .re y => #y
+| .su t => t
+
+@[simp]
+theorem Term.from_action_id {n} : from_action (+0 n) = #n := by
+  simp [from_action, Subst.id]
+
+@[simp]
+theorem Term.from_action_succ {n} : from_action (+1 n) = #(n + 1) := by
+  simp [from_action, Subst.succ]
+
+@[simp]
+theorem Term.from_acton_re {n} : from_action (re n) = #n := by simp [from_action]
+
+@[simp]
+theorem Term.from_action_su {t} : from_action (su t) = t := by simp [from_action]
+
+instance instCoe_SubstActionTerm_Term : Coe (Subst.Action Term) Term where
+  coe := Term.from_action
+
+@[simp]
+def smap (k : Subst.Kind) (lf : Subst.Lift Term k) (f : SplitSubst Term k) : Term -> Term
 | .var x =>
-  match f x with
-  | .re y => .var y
-  | .su t => t
-| .lam A t => .lam (smap lf f A) (smap lf (lf f) t)
-| .bind1 k t => .bind1 k (smap lf (lf f) t)
-| .ctor2 k t1 t2 => .ctor2 k (smap lf f t1) (smap lf f t2)
+  match k with
+  | .re => #(f x)
+  | .su => f x
+| .ctor v ts => .ctor v (λ i => smap k lf f (ts i))
+| .bind v ts t => .bind v (λ i => smap k lf f (ts i)) (smap k lf (lf f) t)
 
 instance SubstMap_Term : SubstMap Term where
   smap := smap
 
-@[simp]
-theorem smap_to_notation : smap Subst.lift σ t = t[σ] := by
+theorem smap_to_notation : smap .su Subst.lift σ t = t[σ] := by
   unfold Subst.apply
   unfold SubstMap.smap
   unfold SubstMap_Term
   simp
 
 @[simp]
-theorem subst_star : ★[σ] = ★ := by
+theorem subst_var : (#x)[σ] = σ x := by
   unfold Subst.apply; simp [SubstMap.smap]
 
 @[simp]
-theorem subst_var :
-  (#x)[σ] = match σ x with | .re y => .var y | .su t => t
+theorem subst_bind
+  : (Term.bind v ts t)[σ] = .bind v (λ i => (ts i)[σ]) t[σ.lift]
+:= by unfold Subst.apply; simp [SubstMap.smap]
+
+@[simp]
+theorem subst_ctor : (Term.ctor v ts)[σ] = .ctor v (λ i => (ts i)[σ]) := by
+  unfold Subst.apply; simp [SubstMap.smap]
+
+@[simp]
+theorem Term.from_action_compose {x} {σ τ : Subst Term}
+  : (from_action (σ x))[τ] = from_action ((σ ∘ τ) x)
 := by
-  unfold Subst.apply; simp [SubstMap.smap]
+  simp [Term.from_action, Subst.compose]
+  generalize zdef : σ x = z
+  cases z <;> simp [Term.from_action]
 
-@[simp]
-theorem subst_lam : (:λ[A] t)[σ] = :λ[A[σ]] t[σ.lift] := by
-  unfold Subst.apply; simp [SubstMap.smap]
-
-@[simp]
-theorem subst_bind1 : (Term.bind1 k t)[σ] = .bind1 k (t[σ.lift]) := by
-  unfold Subst.apply; simp [SubstMap.smap]
-
-@[simp]
-theorem subst_ctor2 : (Term.ctor2 k t1 t2)[σ] = .ctor2 k (t1[σ]) (t2[σ]) := by
-  unfold Subst.apply; simp [SubstMap.smap]
-
-theorem apply_id {t : Term} : t[I] = t := by
+theorem apply_id {t : Term} : t[+0] = t := by
   induction t
   all_goals (simp at * <;> try simp [*])
 
-theorem apply_stable {r : Ren} {σ : Subst Term}
+theorem apply_stable (r : Ren) (σ : Subst Term)
   : r.to = σ -> Ren.apply r = Subst.apply σ
 := by solve_stable r, σ
 
@@ -134,60 +132,12 @@ theorem apply_compose {s : Term} {σ τ : Subst Term} : s[σ][τ] = s[σ ∘ τ]
 instance SubstMapCompose_Term : SubstMapCompose Term where
   apply_compose := apply_compose
 
-namespace LeanSubst.Subst
-  namespace Action
-    @[simp, coe]
-    def coe [Coe A B] : Subst.Action A -> Subst.Action B
-    | .re x => .re x
-    | .su t => .su t
+@[simp]
+theorem ren_apply_to_var : Term.from_action (Ren.to r x) = Term.var (r x) := by
+  simp [Ren.to]
 
-    @[simp]
-    def coe_re [Coe A B] : coe (A := A) (B := B) (#x) = PrefixHash.hash x := by
-      unfold coe; simp
-
-    @[simp]
-    def coe_su [i : Coe A B] :
-      @coe A B i (%t) = PrefixPercent.percent (T := B) (F := Subst.Action) t
-    := by
-      unfold coe; simp
-
-    @[simp]
-    def var : Subst.Action Var -> Nat
-    | .re x => x
-    | .su t => t.out
-  end Action
-end LeanSubst.Subst
-
-instance instCoe_SubstAction_from_Coe [Coe A B] : Coe (Subst.Action A) (Subst.Action B) where
-  coe := Subst.Action.coe
-
-namespace Subst
-  @[simp, coe]
-  def coe [Coe A B] : Subst A -> Subst B
-  | σ, n => σ n
-
-  class CommutesWithSmap (A B) [SubstMap A] [SubstMap B] [c : Coe A B] where
-    coe_commutes : ∀ a (σ : Subst A), Coe.coe (a[σ]) = (Coe.coe a)[@coe _ _ c σ]
-
-  @[simp]
-  theorem coe_cons {a : Subst.Action A} {σ : Subst A} [Coe A B]
-    : coe (a :: σ) = ↑a :: (coe (B := B) σ)
-  := by
-    funext; case _ x =>
-    simp; cases x <;> simp
-
-  @[simp]
-  theorem coe_comp {σ τ : Subst A}
-    [SubstMap A] [SubstMap B] [Coe A B] [i : CommutesWithSmap A B]
-    : coe (σ ∘ τ) = coe (B := B) σ ∘ coe τ
-  := by
-    funext; case _ x =>
-    simp [Subst.compose]
-    generalize zdef : σ x = z at *
-    cases z <;> simp
-    case _ a =>
-      rw [CommutesWithSmap.coe_commutes]
-end Subst
-
-instance instCoe_Subst_from_Coe [Coe A B] : Coe (Subst A) (Subst B) where
-  coe := Subst.coe
+theorem Term.ren_eq_star {r : Ren} : t[r] = ★ -> t = ★ := by
+  intro h; induction t generalizing r <;> simp at *
+  case _ v ts ih =>
+  cases h; case _ h1 h2 =>
+  subst h1; simp at *
