LeanSysF/Typing.lean
@@ -1,36 +1,27 @@
 
 import LeanSubst
 import LeanSysF.Term
+import LeanSysF.Kinding
 
 open LeanSubst
 
-inductive Typing : List Term -> Term -> Term -> Prop where
-| var {Γ T x} :
-  Γ[x]? = .some T ->
-  Typing Γ T ★ ->
+inductive Typing : Ctx Term -> Term -> Term -> Prop where
+| var {Γ : Ctx Term} {T x} :
+  Γ[x] = T ->
+  Γ ⊢ T type ->
   Typing Γ #x T
-| arr {Γ A B} :
-  Typing Γ A ★ ->
-  Typing Γ B ★ ->
-  Typing Γ (A -:> B) ★
 | app {Γ A B f a} :
   Typing Γ f (A -:> B) ->
   Typing Γ a A ->
   Typing Γ (f :@ a) B
 | lam {Γ A B t} :
-  Typing Γ A ★ ->
-  Typing (A::Γ) t (B[S]) ->
+  Γ ⊢ A type ->
+  Typing (A::Γ) t B[+1] ->
   Typing Γ (:λ[A] t) (A -:> B)
-| tvar {Γ x} :
-  Γ[x]? = .some ★ ->
-  Typing Γ #x ★
-| all {Γ P} :
-  Typing (★::Γ) P ★ ->
-  Typing Γ (:∀ P) ★
 | tapp {Γ P P' f a} :
   Typing Γ f (:∀ P) ->
-  Typing Γ a ★ ->
-  P' = P[%a::I] ->
+  Γ ⊢ a type ->
+  P' = P[.su a::+0] ->
   Typing Γ (f :@[a]) P'
 | tlam {Γ P t} :
   Typing (★::Γ) t P ->
@@ -38,165 +29,189 @@ inductive Typing : List Term -> Term -> Term -> Prop where
 
 notation:170 Γ:170 " ⊢ " t:170 " : " A:170 => Typing Γ t A
 
-inductive ActionTyping : List Term -> Subst.Action Term -> Term -> Prop where
-| su :
+theorem Kinding.type_not_term : Γ ⊢ A type -> ¬ (Γ ⊢ A : T) := by
+  intro j1 j2; induction j1
+  all_goals try solve | cases j2
+  case var Γ x h1 =>
+    cases j2; case _ h2 h3 =>
+    rw [h1] at h3; subst h3; cases h2
+
+theorem Typing.term_not_type : Γ ⊢ t : A -> ¬ (Γ ⊢ t type) := by
+  intro j1 j2; induction j1
+  all_goals try solve | cases j2
+  case var Γ T x h1 h2 =>
+    cases j2; case _ h3 =>
+    rw [h1] at h3; subst h3; cases h2
+
+theorem Typing.type_is_type : Γ ⊢ t : A -> Γ ⊢ A type := by
+  intro j; induction j
+  case var j => exact j
+  case app j1 j2 ih1 ih2 =>
+    replace ih1 := Kinding.injection_arrow ih1
+    apply ih1.2
+  case lam j1 j2 ih =>
+    replace ih := Kinding.beta ih j1; simp at ih
+    apply Kinding.arr j1 ih
+  case tapp j1 j2 j3 ih =>
+    cases ih; case _ ih =>
+    replace ih := Kinding.beta ih j2
+    subst j3; apply ih
+  case tlam j ih => apply Kinding.all ih
+
+theorem Typing.rename (Δ : Ctx Term) (r : Ren) :
   Γ ⊢ t : A ->
-  ActionTyping Γ (.su t) A
-| re :
-  Γ ⊢ #x : A ->
-  ActionTyping Γ (.re x) A
-
-notation:170 Γ:170 " ⊢a " t:170 " : " A:170 => ActionTyping Γ t A
-
-def SubstTyping : List Term -> Subst Term -> (Nat -> Term) -> Prop
-| Γ, σ, F => ∀ n, Γ ⊢a σ n : F n
-
-notation:170 Γ:170 " ⊢σ " t:170 " : " A:170 => SubstTyping Γ t A
-
--- theorem typing_renaming_lift {Γ Δ} A {r : Ren} :
---   (∀ x T, Γ ⊢ #x : T -> Δ ⊢ #(r x) : T) ->
---   ∀ x T, (A::Γ) ⊢ #x : T -> (A::Δ) ⊢ #(r.lift x) : T
--- := by
--- intro h x T j
--- simp [Ren.lift]; cases x <;> simp at *
--- case _ =>
---   cases j; case _ j =>
---   apply Typing.var
---   simp at *; subst j; rfl
--- case _ x =>
---   cases j; case _ j =>
---   simp at j; apply Typing.var
---   simp; have lem := h x T (Typing.var j)
---   cases lem; case _ lem => ↑x
---   apply lem
-
-theorem typing_renaming_lift {Γ Δ : List Term} (A : Term) {σ : Subst Var } :
-  (∀ x (T : Term), Γ[x]? = .some T -> Δ[(σ x).var]? = .some (T[Coe.coe σ])) ->
-  ∀ x (T : Term), (A :: Γ)[x]? = .some T
-    -> (A[Coe.coe σ] :: Δ)[(σ.lift x).var]? = .some (T[Coe.coe σ.lift])
+  (∀ x T, Γ[x] = T -> Δ[r x] = T[r]) ->
+  Δ ⊢ t[r] : A[r]
 := by
-  sorry
+  intro j h
+  induction j generalizing Δ r
+  case var Γ T x j1 j2 =>
+    simp; apply Typing.var
+    apply h x T j1
+    apply Kinding.rename _ _ j2 h
+  case lam Γ A B t j1 j2 ih =>
+    replace ih := ih (A[r]::Δ) r.lift (Ctx.rename_lift A h)
+    rw [Ren.to_lift] at ih; simp at ih
+    simp; apply Typing.lam
+    apply Kinding.rename _ _ j1 h
+    simp; apply ih
+  case app Γ A B f a j1 j2 ih1 ih2 =>
+    replace ih1 := ih1 Δ r h; simp at ih1
+    simp; apply Typing.app
+    apply ih1
+    apply ih2 Δ r h
+  case tlam Γ P t j ih =>
+    replace ih := ih (★[r]::Δ) r.lift (Ctx.rename_lift ★ h)
+    rw [Ren.to_lift] at ih; simp at ih
+    simp; apply Typing.tlam ih
+  case tapp Γ P P' f a j1 j2 j3 ih =>
+    replace ih := ih Δ r h; simp at ih
+    simp; apply Typing.tapp ih
+    apply Kinding.rename _ _ j2 h
+    subst j3; simp
 
-theorem typing_weaken {Γ t A} Δ (σ : Subst Var) :
+theorem Typing.weaken B : Γ ⊢ t : A -> (B::Γ) ⊢ t[+1] : A[+1] := by
+  intro j
+  have lem := rename (B::Γ) (· + 1) j
+  simp at lem; exact lem
+
+theorem Typing.subst_lift {σ : Subst Term} {Γ Δ : Ctx Term} A :
+  (∀ x T t, Γ[x] = T -> Γ ⊢ T type -> σ x = su t -> Δ ⊢ t : T[σ]) ->
+  ∀ x T t, (A::Γ)[x] = T -> (A::Γ) ⊢ T type -> σ.lift x = su t -> (A[σ]::Δ) ⊢ t : T[σ.lift]
+:= by
+  intro h1 x T t h2 h3 h4
+  cases x <;> simp at *
+  case _ x =>
+  unfold Subst.compose at h4; simp at h4
+  generalize zdef : σ x = z at *
+  cases z <;> simp at *
+  case _ s =>
+  subst h4; subst h2
+  have lem := h1 x Γ[x] s rfl (Kinding.strengthen h3) zdef
+  have lem2 := weaken (A[σ]) lem
+  simp at *; apply lem2
+
+theorem Typing.subst (Δ : Ctx Term) (σ : Subst Term) :
   Γ ⊢ t : A ->
-  (∀ x (T : Term), Γ[x]? = .some T -> Δ[(σ x).var]? = .some (T[Coe.coe σ])) ->
+  (∀ x T y, Γ[x] = T -> σ x = re y -> Δ[y] = T[σ]) ->
+  (∀ x t, Γ[x] = ★ -> σ x = su t -> Δ ⊢ t type) ->
+  (∀ x T t, Γ[x] = T -> Γ ⊢ T type -> σ x = su t -> Δ ⊢ t : T[σ]) ->
   Δ ⊢ t[σ] : A[σ]
 := by
-intro j h
-induction j generalizing Δ σ
-case var Γ T x j1 j2 ih =>
-  simp; generalize zdef : σ x = z at *
-  cases z <;> simp
-  case _ y =>
-    apply Typing.var
-    have lem := h x T j1
-    rw [zdef] at lem; simp at lem
-    apply lem
-    apply ih _ _ h
-  case _ t =>
-    cases t; case _ t p =>
-    cases p; case _ y =>
-    simp; apply Typing.var
-    have lem := h x T j1
-    rw [zdef] at lem; simp at lem
-    apply lem
-    apply ih _ _ h
-case arr j1 j2 ih1 ih2 =>
-  simp; apply Typing.arr
-  apply ih1 _ _ h
-  apply ih2 _ _ h
-case app j1 j2 ih1 ih2 =>
-  simp; apply Typing.app
-  apply ih1 _ _ h
-  apply ih2 _ _ h
-case lam Γ A B t j1 j2 ih1 ih2 =>
-  simp; apply Typing.lam
-  apply ih1 _ _ h
-  replace ih2 := ih2 (A[σ] :: Δ) (σ.lift) (typing_renaming_lift A h)
-  simp at ih2; simp
-  apply ih2
-case tvar Γ x j =>
-  simp; generalize zdef : σ x = z at *
-  cases z <;> simp
-  case _ y =>
-    apply Typing.tvar
-    have lem := h x ★ j
-    rw [zdef] at lem; simp at lem
-    apply lem
-  case _ t =>
-    cases t; case _ t p =>
-    cases p; case _ y =>
-    simp; apply Typing.tvar
-    have lem := h x ★ j
-    rw [zdef] at lem; simp at lem
-    apply lem
-case all j ih =>
-  simp; apply Typing.all
-  replace ih := ih (★ :: Δ) σ.lift (typing_renaming_lift ★ h)
-  simp at ih; apply ih
-case tapp j1 j2 j3 ih1 ih2 =>
-  simp; apply Typing.tapp
-  apply ih1 _ _ h
-  apply ih2 _ _ h
-  rw [j3]; simp
-case tlam j ih =>
-  simp; apply Typing.tlam
-  replace ih := ih (★ :: Δ) σ.lift (typing_renaming_lift ★ h)
-  simp at ih; apply ih
+  intro j h1 h2 h3
+  induction j generalizing Δ σ
+  case var Γ T x j1 j2 =>
+    simp; generalize zdef : σ x = z
+    cases z <;> simp
+    case _ z =>
+      have lem := h1 x T z j1 zdef
+      apply Typing.var lem
+      apply Kinding.subst Δ σ j2 h1 h2
+    case _ t => apply h3 x T t j1 j2 zdef
+  case lam Γ A B t j1 j2 ih =>
+    have lem := Kinding.subst Δ σ j1 h1 h2
+    simp; apply Typing.lam lem
+    replace ih := ih (A[σ]::Δ) σ.lift
+      (Ctx.subst_re_lift A h1)
+      (Kinding.subst_lift A h2)
+      (subst_lift A h3)
+    simp at *; apply ih
+  case app ih1 ih2 =>
+    replace ih1 := ih1 Δ σ h1 h2 h3; simp at ih1
+    simp; apply Typing.app
+    apply ih1
+    apply ih2 Δ σ h1 h2 h3
+  case tlam ih =>
+    simp; apply Typing.tlam
+    replace ih := ih (★[σ]::Δ) σ.lift
+      (Ctx.subst_re_lift ★ h1)
+      (Kinding.subst_lift ★ h2)
+      (subst_lift ★ h3)
+    simp at *; apply ih
+  case tapp j1 j2 j3 ih =>
+    replace ih := ih Δ σ h1 h2 h3; simp at ih
+    simp; apply Typing.tapp
+    apply ih; apply Kinding.subst Δ σ j2 h1 h2
+    subst j3; simp
 
--- theorem typing_subst_lift {Γ Δ} A {σ : Subst Term} :
---   (∀ x T, Γ ⊢ #x : T -> Δ ⊢ ↑(σ x) : T) ->
---   ∀ x T, (A::Γ) ⊢ #x : T -> (A::Δ) ⊢ ↑(σ.lift x) : T
--- := by
--- intro h x T j
--- cases j; case _ j =>
--- cases x <;> simp at *
--- case _ => subst j; apply Typing.var; simp
--- case _ x =>
---   have h' := h _ _ (Typing.var j)
---   have lem := typing_weaken (A :: Δ) (λ x => x + 1) h' (by {
---     intro x T j2; simp
---     apply Typing.var; simp
---     cases j2; simp [*]
---   }); simp at lem
---   unfold Subst.compose; simp
---   generalize zdef : σ x = z at *
---   cases z <;> simp at *
---   apply lem
---   rw [SubstMapStable.apply_stable (σ := S) (by rw [to_S])] at lem
---   apply lem
+theorem Typing.beta :
+  (A::Γ) ⊢ t : T ->
+  Γ ⊢ a : A ->
+  Γ ⊢ t[su a::+0] : T[su a::+0]
+:= by
+  intro j1 j2
+  apply subst Γ (su a::+0) j1
+  case _ =>
+    intro x T y h1 h2
+    cases x <;> simp at *
+    case _ x =>
+    subst h1; subst h2; simp
+  case _ =>
+    intro x s h1 h2
+    cases x <;> simp at *
+    replace h1 := Term.ren_eq_star h1
+    subst h1; subst h2
+    have lem := type_is_type j2
+    cases lem
+  case _ =>
+    intro x S s h1 h2 h3
+    cases x <;> simp at *
+    subst h1; subst h3; simp
+    apply j2
 
--- theorem typing_subst {Γ t A} Δ (σ : Subst Term) :
---   Γ ⊢ t : A ->
---   (∀ x T, Γ ⊢ #x : T -> Δ ⊢ ↑(σ x) : T) ->
---   Δ ⊢ t[σ] : A
--- := by
--- intro j h
--- induction j generalizing Δ σ
--- case var T x j =>
---   replace h := h x T; simp
---   generalize zdef : σ x = z at *
---   cases z <;> simp at *
---   all_goals apply h; apply Typing.var j
--- case app j1 j2 ih1 ih2 =>
---   simp; apply Typing.app
---   apply ih1 _ _ h
---   apply ih2 _ _ h
--- case lam j ih =>
---   simp; apply Typing.lam
---   replace ih := ih _ _ (typing_subst_lift _ h)
---   simp at ih; apply ih
+theorem Typing.beta_type :
+  (★::Γ) ⊢ t : T ->
+  Γ ⊢ a type ->
+  Γ ⊢ t[su a::+0] : T[su a::+0]
+:= by
+  intro j1 j2
+  apply subst Γ (su a::+0) j1
+  case _ =>
+    intro x A y h1 h2
+    cases x <;> simp at *
+    case _ x =>
+    subst h1; subst h2; simp
+  case _ =>
+    intro x s h1 h2
+    cases x <;> simp at *
+    subst h2; apply j2
+  case _ =>
+    intro x S s h1 h2 h3
+    cases x <;> simp at *
+    subst h1; subst h3
+    cases h2
 
--- theorem typing_beta {Γ A B b t} : (A::Γ) ⊢ b : B -> Γ ⊢ t : A -> Γ ⊢ b[.su t::I] : B := by
--- intro j1 j2
--- apply typing_subst Γ (.su t::I) j1 (λ x T h => by {
---   simp; cases x <;> simp
---   case _ =>
---     cases h; case _ h =>
---     simp at h; subst h
---     apply j2
---   case _ x =>
---     cases h; case _ h =>
---     simp at h
---     apply Typing.var h
--- })
+theorem Typing.lam_inv :
+  Γ ⊢ :λ[C] t : (A -:> B) ->
+  (A::Γ) ⊢ t : B[+1]
+:= by
+  intro j
+  generalize zdef : (:λ[C] t) = z at j
+  generalize wdef : (A -:> B) = w at j
+  cases j
+  all_goals try solve | (try injection zdef; try injection wdef)
+  injection zdef with _ e1 e2; subst e2
+  injection wdef with _ e3
+  case _ j _ =>
+  simp at *; cases e3; case _ e1 e2 =>
+  subst e1; subst e2; exact j
