LeanSysF/CtxWf.lean
@@ -1,0 +1,15 @@
+
+import LeanSubst
+import LeanSysF.Term
+import LeanSysF.Kinding
+
+open LeanSubst
+
+inductive CtxWf : Ctx Term -> Prop where
+| nil : CtxWf []
+| cons :
+  Γ ⊢ A type ->
+  CtxWf Γ ->
+  CtxWf (A::Γ)
+
+notation:170 "⊢ " Γ:170 => CtxWf Γ
