LeanSysF/FreeVar.lean
@@ -1,0 +1,106 @@
+
+import LeanSubst
+import LeanSysF.Utility
+import LeanSysF.Term
+
+open LeanSubst
+
+inductive FV : Term -> Nat -> Prop
+| var : FV #x x
+| ctor {i : Fin v.arity} {ts : Fin v.arity -> Term} : FV (ts i) x -> FV (.ctor v ts) x
+| bind1 {i : Fin v.arity} {ts : Fin v.arity -> Term} : FV (ts i) x -> FV (.bind v ts t) x
+| bind2 : FV t (x + 1) -> FV (.bind v ts t) x
+
+instance : Membership Nat Term where
+  mem := FV
+
+theorem FV.found : x ∈ #x := by simp [Membership.mem]; apply FV.var
+
+@[simp]
+theorem FV.ctor_inj : x ∈ (Term.ctor v ts) <-> ∃ i, x ∈ (ts i) := by
+  apply Iff.intro
+  case _ =>
+    intro h; simp [Membership.mem] at *
+    cases h; case _ i h =>
+    exists i
+  case _ =>
+    intro h; simp [Membership.mem] at *
+    cases h; case _ i h =>
+    apply FV.ctor h
+
+@[simp]
+theorem FV.bind_inj : x ∈ (Term.bind v ts t) <-> (∃ i, x ∈ (ts i)) ∨ x + 1 ∈ t := by
+  apply Iff.intro
+  case _ =>
+    intro h; cases h
+    case _ i h => apply Or.inl; exists i
+    case _ h => apply Or.inr; apply h
+  case _ =>
+    intro h; cases h
+    case _ h =>
+      cases h; case _ i h =>
+      apply FV.bind1 h
+    case _ h => apply FV.bind2 h
+
+theorem lift_iterated_succ_is_re
+  : ((Subst.lift (T := Term))^[n]) +1 y = z -> ∃ i, z = re i
+:= by
+  intro h
+  induction n generalizing y z
+  case zero =>
+    simp at h; cases z
+    case _ i =>
+      injection h with e; subst e
+      exists (y + 1)
+    case _ t => injection h
+  case succ n ih =>
+    simp at h
+    cases y <;> simp at h
+    case zero => exists 0; subst h; rfl
+    case succ y =>
+      unfold Subst.compose at h; simp at h
+      generalize udef : ((Subst.lift (T := Term))^[n]) +1 y = u at *
+      cases u <;> simp at *
+      case _ i => exists (i + 1); subst h; rfl
+      case _ t =>
+        replace ih := @ih y; cases ih; case _ i ih =>
+        rw [ih] at udef; injection udef
+
+theorem FV.var_not_in_one_more {t : Term} : ¬ (x ∈ t[((Subst.lift)^[x]) +1]) := by
+  intro h
+  induction t generalizing x <;> simp at *
+  case var y =>
+    induction x generalizing y <;> simp at *
+    case _ => cases h
+    case _ n ih =>
+      cases y <;> simp at *
+      case _ => cases h
+      case _ y =>
+        unfold Subst.compose at h; simp at h
+        generalize zdef : (((Subst.lift (T := Term))^[n]) +1 y) = z at *
+        cases z <;> simp at *
+        case _ z =>
+          replace ih := ih y
+          cases h; rw [zdef] at ih; simp at ih
+          apply ih; apply FV.var
+        case _ t =>
+          have lem := lift_iterated_succ_is_re zdef
+          cases lem; case _ i lem =>
+          injection lem
+  case bind v ts t ih1 ih2 =>
+    cases h
+    case _ h =>
+      cases h; case _ i h =>
+      replace ih1 := @ih1 i x
+      apply ih1 h
+    case _ h =>
+      replace ih2 := @ih2 (x + 1); simp at ih2
+      apply ih2 h
+  case ctor v ts ih =>
+    cases h; case _ i h =>
+    apply ih i h
+
+theorem FV.zero_not_in_succ {t : Term} : ¬ (0 ∈ t[+1]) := by
+  intro j
+  have lem := @var_not_in_one_more 0 t; simp at lem
+  apply lem j
