LeanSysF/Kinding.lean
@@ -1,0 +1,187 @@
+
+import LeanSubst
+import LeanSysF.Term
+import LeanSysF.FreeVar
+
+open LeanSubst
+
+inductive Kinding : Ctx Term -> Term -> Prop where
+| var {Γ : Ctx Term} {x} :
+  Γ[x] = ★ ->
+  Kinding Γ #x
+| arr {Γ A B} :
+  Kinding Γ A ->
+  Kinding Γ B ->
+  Kinding Γ (A -:> B)
+| all {Γ P} :
+  Kinding (★::Γ) P ->
+  Kinding Γ (:∀ P)
+
+notation:170 Γ:170 " ⊢ " A:170 " type" => Kinding Γ A
+
+theorem Ctx.strong_rename_lift {A : Term} {Δ Γ : Ctx Term} {r : Ren} B :
+  (∀ x T, x + 1 ∈ A -> Γ[x] = T -> Δ[r x] = T[r]) ->
+  ∀ x T, x ∈ A -> (B::Γ)[x] = T -> (B[r]::Δ)[r.lift x] = T[r.lift]
+:= by
+  intro h1 x T h2 h3
+  cases x <;> simp at *
+  case zero =>
+    subst h3; simp [Ren.lift]
+    rw [Ren.to_lift]; simp
+  case succ x =>
+    replace h1 := h1 x h2
+    subst h3; simp [Ren.lift]
+    rw [Ren.to_lift]; rw [h1]; simp
+
+theorem Ctx.rename_lift {Δ Γ : Ctx Term} {r : Ren} B :
+  (∀ x T, Γ[x] = T -> Δ[r x] = T[r]) ->
+  ∀ x T, (B::Γ)[x] = T -> (B[r]::Δ)[r.lift x] = T[r.lift]
+:= by
+  intro h1 x T h3
+  cases x <;> simp at *
+  case zero =>
+    subst h3; simp [Ren.lift]
+    rw [Ren.to_lift]; simp
+  case succ x =>
+    replace h1 := h1 x
+    subst h3; simp [Ren.lift]
+    rw [Ren.to_lift]; rw [h1]; simp
+
+theorem Ctx.subst_re_lift {Γ Δ : Ctx Term} A {σ : Subst Term} :
+  (∀ x T y, Γ[x] = T -> σ x = re y -> Δ[y] = T[σ]) ->
+  ∀ x T y, (A::Γ)[x] = T -> σ.lift x = re y -> (A[σ]::Δ)[y] = T[σ.lift]
+:= by
+  intro h1 x T y h2 h3
+  cases x <;> simp at *
+  case zero => subst h2; subst h3; simp
+  case succ x =>
+    simp [Subst.compose] at h3
+    generalize zdef : σ x = z at *
+    cases z <;> simp at h3
+    case _ z =>
+    subst h3
+    replace h1 := h1 x Γ[x] z rfl zdef
+    subst h2; simp; rw [h1]; simp
+
+theorem Kinding.strong_rename {Γ A} (Δ : Ctx Term) (r : Ren) :
+  Γ ⊢ A type ->
+  (∀ x T, x ∈ A -> Γ[x] = T -> Δ[r x] = T[r]) ->
+  Δ ⊢ A[r] type
+:= by
+  intro j h
+  induction j generalizing Δ r
+  case var Γ x j =>
+    replace h := h x ★ FV.found j; simp at h
+    simp; apply Kinding.var h
+  case arr Γ A B j1 j2 ih1 ih2 =>
+    have h1 := λ x T (e : x ∈ A) => h x T (by simp; apply Or.inl e)
+    have h2 := λ x T (e : x ∈ B) => h x T (by simp; apply Or.inr e)
+    simp; apply Kinding.arr
+    apply ih1 Δ r h1
+    apply ih2 Δ r h2
+  case all Γ P j ih =>
+    have h2 : ∀ x T, x + 1 ∈ P -> Γ[x] = T -> Δ[r x] = T[r] := by
+      intro x T q1 q2; simp at h
+      replace h := h x q1; subst q2
+      apply h
+    simp; apply Kinding.all
+    have lem1 := Ctx.strong_rename_lift ★ h2; simp at lem1
+    have lem2 := ih (★::Δ) r.lift; simp at lem2
+    replace lem2 := lem2 lem1
+    rw [Ren.to_lift] at lem2; simp at lem2; exact lem2
+
+theorem Kinding.rename {Γ A} (Δ : Ctx Term) (r : Ren) :
+  Γ ⊢ A type ->
+  (∀ x T, Γ[x] = T -> Δ[r x] = T[r]) ->
+  Δ ⊢ A[r] type
+:= by
+  intro j h
+  apply strong_rename _ _ j _
+  intro x T h1 h2
+  apply h x T h2
+
+theorem Kinding.weaken : Γ ⊢ A type -> (P::Γ) ⊢ A[+1] type := by
+  intro j
+  have lem := rename (P::Γ) (· + 1) j
+  simp at lem; exact lem
+
+theorem Kinding.strengthen : (P::Γ) ⊢ A[+1] type -> Γ ⊢ A type := by
+  intro j
+  have lem := strong_rename Γ (· - 1) j (by {
+    intro x T h1 h2
+    cases x <;> simp at *
+    case zero => exfalso; apply FV.zero_not_in_succ h1
+    case succ x => subst h2; simp
+  })
+  simp at lem; apply lem
+
+theorem Kinding.subst_lift {Γ Δ : Ctx Term} A {σ : Subst Term} :
+  (∀ x t, Γ[x] = ★ -> σ x = su t -> Δ ⊢ t type) ->
+  ∀ x t, (A::Γ)[x] = ★ -> σ.lift x = su t -> (A[σ]::Δ) ⊢ t type
+:= by
+  intro h1 x t h2 h3
+  cases x <;> simp at *
+  case _ x =>
+  replace h2 := Term.ren_eq_star h2
+  simp [Subst.compose] at h3
+  generalize zdef : σ x = z at *
+  cases z <;> simp at *
+  case _ s =>
+  subst h3
+  replace h1 := h1 x s h2 zdef
+  have lem := rename (A[σ]::Δ) (· + 1) h1
+  simp at lem; exact lem
+
+theorem Kinding.subst {Γ A} (Δ : Ctx Term) (σ : Subst Term) :
+  Γ ⊢ A type ->
+  (∀ x T y, Γ[x] = T -> σ x = re y -> Δ[y] = T[σ]) ->
+  (∀ x t, Γ[x] = ★ -> σ x = su t -> Δ ⊢ t type) ->
+  Δ ⊢ A[σ] type
+:= by
+  intro j h1 h2
+  induction j generalizing Δ σ
+  case var Γ x j =>
+    simp; generalize zdef : σ x = z at *
+    cases z <;> simp at *
+    case _ y =>
+      apply Kinding.var
+      have lem := h1 x ★ y j zdef; simp at lem
+      exact lem
+    case _ t => apply h2 x t j zdef
+  case arr Γ A B j1 j2 ih1 ih2 =>
+    simp; apply Kinding.arr
+    apply ih1 Δ σ h1 h2
+    apply ih2 Δ σ h1 h2
+  case all Γ P j ih =>
+    -- TODO: Why does Lean unfold Subst.lift?
+    have lem0 : ★[σ] = ★ := by simp
+    have lem1 := Ctx.subst_re_lift ★ h1; rw [lem0] at lem1
+    have lem2 := Kinding.subst_lift ★ h2; rw [lem0] at lem2
+    simp; apply Kinding.all
+    have lem3 := ih (★::Δ) σ.lift lem1 lem2; simp at lem3
+    exact lem3
+
+theorem Kinding.beta : (A::Γ) ⊢ P type -> Γ ⊢ B type -> Γ ⊢ P[su B::+0] type := by
+  intro j1 j2
+  apply subst Γ (su B::+0) j1
+  case _ =>
+    intro x T y h1 h2
+    cases x <;> simp at *
+    case _ n => subst h1; subst h2; simp
+  case _ =>
+    intro x t h1 h2
+    cases x <;> simp at *
+    case zero =>
+      replace h1 := Term.ren_eq_star h1
+      subst h1; subst h2; apply j2
+
+theorem Kinding.injection_arrow : Γ ⊢ (A -:> B) type -> Γ ⊢ A type ∧ Γ ⊢ B type := by
+  intro j; generalize zdef : A -:> B = z at *
+  cases j; all_goals injection zdef
+  case arr A' B' j1 j2 e1 e2 =>
+    have lem1 : ∀ x, (λ i => mk2 A B i) x = (λ i => mk2 A' B' i) x := by
+      intro x; rw [e2]
+    have lem2 := lem1 0; simp [mk2] at lem2
+    have lem3 := lem1 1; simp [mk2] at lem3
+    subst lem2; subst lem3
+    apply And.intro j1 j2
