LeanSysF/Preservation.lean
@@ -1,0 +1,96 @@
+import LeanSubst
+import LeanSysF.Term
+import LeanSysF.Kinding
+import LeanSysF.Typing
+import LeanSysF.Reduction
+import LeanSysF.Progress
+
+open LeanSubst
+
+theorem preservation_step : Γ ⊢ t : A -> t ~> t' -> Γ ⊢ t' : A := by
+  intro j r
+  induction j generalizing t'
+  case var => cases r
+  case app Γ A B f a j1 j2 ih1 ih2 =>
+    generalize zdef : f :@ a = z at *
+    cases r; all_goals try solve | cases zdef
+    case beta A' b' t' =>
+      injection zdef with _ e; simp at e
+      cases e; case _ e1 e2 =>
+      subst e1; subst e2
+      replace j1 := Typing.lam_inv j1
+      replace j1 := Typing.beta j1 j2; simp at j1
+      apply j1
+    case ctor v i ts ts' h r =>
+      injection zdef with e1 e2; subst e1; subst e2
+      simp at *
+      cases i; case _ i p =>
+      cases i; case _ =>
+        simp at *; subst h
+        replace ih1 := ih1 r
+        rw [<-mk2_eta (t := ts')]
+        apply Typing.app ih1 j2
+      case _ i =>
+      cases i; case _ i =>
+        simp at *; subst h
+        replace ih2 := ih2 r
+        rw [<-mk2_eta (t := ts')]
+        apply Typing.app j1 ih2
+      case _ i =>
+        simp [Variant.arity] at p
+        omega
+  case lam Γ A B t j1 j2 ih =>
+    cases r
+    case bind1 i ts h r =>
+      cases i; case _ i p =>
+      cases i <;> simp at *
+      case _ =>
+        have lem := Kinding.value j1
+        exfalso; apply Value.sound lem _ r
+      case _ n => simp at p
+    case bind2 t' r =>
+      replace ih := ih r
+      apply Typing.lam j1 ih
+  case tapp Γ P P' f a j1 j2 j3 ih =>
+    generalize zdef : f :@[a] = z at *
+    cases r; all_goals try solve | cases zdef
+    case tbeta b' t' =>
+      injection zdef with _ e; simp at e
+      cases e; case _ e1 e2 =>
+      subst e1; subst e2
+      cases j1; case _ j1 =>
+      have lem := Typing.beta_type j1 j2
+      subst j3; apply lem
+    case ctor v i ts ts' h r =>
+      injection zdef with e1 e2; subst e1; subst e2
+      simp at *
+      cases i; case _ i p =>
+      cases i; case _ =>
+        simp at *; subst h
+        replace ih := ih r
+        rw [<-mk2_eta (t := ts')]
+        apply Typing.tapp ih j2 j3
+      case _ i =>
+      cases i; case _ i =>
+        simp at *; subst h
+        have lem := Kinding.value j2
+        replace lem := Value.sound lem
+        exfalso; apply lem _ r
+      case _ i =>
+        simp [Variant.arity] at p
+        omega
+  case tlam Γ P t j ih =>
+    cases r
+    case bind1 i ts' h r =>
+      cases i; case _ i p =>
+      simp [Variant.arity] at p
+    case bind2 t' r =>
+      replace ih := ih r
+      apply Typing.tlam ih
+
+theorem preservation : Γ ⊢ t : A -> t ~>* t' -> Γ ⊢ t' : A := by
+  intro j r
+  induction r
+  case _ => exact j
+  case _ y z r1 r2 ih =>
+    apply preservation_step ih r2
