LeanSysF/Progress.lean
@@ -1,0 +1,224 @@
+import LeanSubst
+import LeanSysF.Term
+import LeanSysF.Kinding
+import LeanSysF.Typing
+import LeanSysF.Reduction
+
+open LeanSubst
+
+@[simp]
+def Term.is_lam : Term -> Bool
+| .bind .lam _ _ => true
+| _ => false
+
+@[simp]
+def Term.is_tlam : Term -> Bool
+| .bind .tlam _ _ => true
+| _ => false
+
+inductive Value : Term -> Prop where
+| var : Value #x
+| ctor {ts : Fin v.arity -> Term} :
+  ((h : v = .app) -> !(ts (by subst h; exact 0)).is_lam) ->
+  ((h : v = .tapp) -> !(ts (by subst h; exact 0)).is_tlam) ->
+  (∀ i, Value (ts i)) ->
+  Value (.ctor v ts)
+| bind {ts : Fin v.arity -> Term} :
+  (∀ i, Value (ts i)) ->
+  Value t ->
+  Value (.bind v ts t)
+
+theorem Value.mk1 : Value t -> ∀ (a : Fin 1), Value (mk1 t a) := by
+  intro v a
+  cases a; case _ x p =>
+  cases x; exact v
+  omega
+
+theorem Value.mk2 {ts : Fin 2 -> Term} :
+  Value (ts 0) ->
+  Value (ts 1) ->
+  ∀ (a : Fin 2), Value (ts a)
+:= by
+  intro v1 v2 a
+  cases a; case _ x p =>
+  cases x; exact v1; case _ x =>
+  cases x; exact v2; case _ x =>
+  omega
+
+theorem Value.sound : Value t -> ∀ t', ¬ (t ~> t') := by
+  intro h
+  induction h
+  case var => intro t' r; cases r
+  case ctor v ts j1 j2 j3 ih =>
+    intro t' r
+    cases r
+    case _ => simp at j1
+    case _ => simp at j2
+    case _ i ts' h r => apply ih i _ r
+  case bind t v ts j1 j2 ih1 ih2 =>
+    intro t' r
+    cases r
+    case _ i ts' h r => apply ih1 i _ r
+    case _ t' r => apply ih2 _ r
+
+theorem Kinding.value : Γ ⊢ A type -> Value A := by
+  intro j; induction j
+  case var => apply Value.var
+  case arr ih1 ih2 =>
+    apply Value.ctor
+    all_goals simp [*]
+  case all ih =>
+    apply Value.bind
+    all_goals simp [*]
+
+theorem progress t : Value t ∨ (∃ t', t ~> t') := by
+  induction t
+  case var => apply Or.inl; apply Value.var
+  case ctor v ts ih =>
+    cases v <;> simp at *
+    case _ =>
+      apply Or.inl; apply Value.ctor
+      all_goals simp
+    case _ =>
+      cases ih; case _ ih1 ih2 =>
+      cases ih1
+      case _ ih1 =>
+        cases ih2
+        case _ ih2 =>
+          generalize zdef : ts 0 = z
+          cases z
+          case bind v ts' t' =>
+            cases v
+            case lam =>
+              apply Or.inr
+              generalize adef : ts 1 = a at *
+              exists (t'[su a::+0])
+              rw [<-mk2_eta (t := ts)]
+              rw [zdef, adef]
+              rw [<-mk1_eta (t := ts')]
+              apply Red.beta
+            all_goals solve | (
+              apply Or.inl; apply Value.ctor
+              simp; rw [zdef]; simp
+              apply Value.mk2 ih1 ih2)
+          all_goals solve | (
+            rw [zdef] at ih1
+            apply Or.inl
+            apply Value.ctor
+            simp; rw [zdef]
+            simp; simp [*])
+        case _ ih2 =>
+          cases ih2; case _ t' ih2 =>
+          apply Or.inr
+          exists ((ts 0) :@ t')
+          apply Red.ctor (i := 1)
+          all_goals simp [*]
+      case _ ih1 =>
+        cases ih1; case _ t' ih1 =>
+        apply Or.inr
+        exists (t' :@ (ts 1))
+        apply Red.ctor (i := 0)
+        all_goals simp [*]
+    case _ =>
+      cases ih; case _ ih1 ih2 =>
+      cases ih1
+      case _ ih1 =>
+        cases ih2
+        case _ ih2 =>
+          generalize zdef : ts 0 = z
+          cases z
+          case bind v ts' t' =>
+            cases v
+            case tlam =>
+              apply Or.inr
+              generalize adef : ts 1 = a at *
+              exists (t'[su a::+0])
+              rw [<-mk2_eta (t := ts)]
+              rw [zdef, adef]; simp
+              apply Red.tbeta
+            all_goals solve | (
+              apply Or.inl; apply Value.ctor
+              simp; simp; rw [zdef]
+              apply Value.mk2 ih1 ih2)
+          all_goals solve | (
+            rw [zdef] at ih1
+            apply Or.inl
+            apply Value.ctor
+            simp; simp; rw [zdef]
+            simp [*])
+        case _ ih2 =>
+          cases ih2; case _ t' ih2 =>
+          apply Or.inr
+          exists ((ts 0) :@[t'])
+          apply Red.ctor (i := 1)
+          all_goals simp [*]
+      case _ ih1 =>
+        cases ih1; case _ t' ih1 =>
+        apply Or.inr
+        exists (t' :@[ts 1])
+        apply Red.ctor (i := 0)
+        all_goals simp [*]
+    case _ =>
+      cases ih; case _ ih1 ih2 =>
+      cases ih1
+      case _ ih1 =>
+        cases ih2
+        case _ ih2 =>
+          apply Or.inl
+          apply Value.ctor
+          all_goals simp [*]
+        case _ ih2 =>
+          cases ih2; case _ t' r =>
+          apply Or.inr
+          exists ((ts 0) -:> t')
+          apply Red.ctor (i := 1)
+          all_goals simp [*]
+      case _ ih1 =>
+        cases ih1; case _ t' r =>
+        apply Or.inr
+        exists (t' -:> (ts 1))
+        apply Red.ctor (i := 0)
+        all_goals simp [*]
+  case bind v ts t ih1 ih2 =>
+    cases v <;> simp at *
+    case _ =>
+      cases ih1
+      case _ ih1 =>
+        cases ih2
+        case _ ih2 =>
+          apply Or.inl
+          apply Value.bind
+          all_goals simp [*]
+        case _ ih2 =>
+          cases ih2; case _ t' r =>
+          apply Or.inr
+          exists (:λ[ts 0] t'); simp
+          apply Red.bind2 r
+      case _ ih1 =>
+        cases ih1; case _ t' r =>
+        apply Or.inr
+        exists (:λ[t'] t)
+        apply Red.bind1 (i := 0)
+        all_goals simp [*]
+    case _ =>
+      cases ih2
+      case _ ih2 =>
+        apply Or.inl
+        apply Value.bind
+        all_goals simp [*]
+      case _ ih2 =>
+        cases ih2; case _ t' r =>
+        apply Or.inr
+        exists (Λ t')
+        apply Red.bind2 r
+    case _ =>
+      cases ih2
+      case _ ih2 =>
+        apply Or.inl
+        apply Value.bind
+        all_goals simp [*]
+      case _ ih2 =>
+        cases ih2; case _ t' r =>
+        apply Or.inr
+        exists (:∀ t')
+        apply Red.bind2 r
