LeanSysF/Utility.lean
@@ -1,0 +1,12 @@
+
+@[simp]
+def iterate (f : T -> T) : Nat -> T -> T
+| 0 => λ x => x
+| n + 1 => λ x => f $ (iterate f n) x
+
+notation f "^[" n "]" => iterate f n
+
+@[simp]
+theorem iterate_succ {x : Nat} : ((· + 1)^[n]) x = x + n := by
+  induction n <;> simp at *
+  case succ n ih => rw [ih]; omega
