README.md
@@ -1,1 +1,10 @@
 # lean-sysf
+
+
+# Notes
+
+strengthening of kinding is needed for substitution of typing
+
+this should be avoidable by annotating variables and context entries with their sort (term or type)
+
+but non-annotated variables is "closer" to the original setup of System F
